TT-model/safety.lean
@@ -1,0 +1,179 @@
+import «TT-model».syntactics
+import «TT-model».reduction
+import «TT-model».typing
+
+open Nat
+open Term
+
+set_option autoImplicit false
+set_option pp.fieldNotation false
+
+variable [LevelClass]
+
+/-*----------------------
+  Well-scoped renamings
+----------------------*-/
+
+def wRename ξ Γ Δ := ∀ x A, Γ ∋ x ∶ A → Δ ∋ ξ x ∶ rename ξ A
+notation:40 Δ:41 "⊢" ξ:41 "∶" Γ:41 => wRename ξ Γ Δ
+
+theorem wRenameLift {ξ : ℕ → ℕ} {Γ Δ A}
+  (h : Δ ⊢ ξ ∶ Γ) :
+  Δ ∷ (rename ξ A) ⊢ lift ξ ∶ Γ ∷ A := by
+  intro x B mem
+  cases mem with
+  | here => apply inHere; simp [renameComp]; rfl
+  | there => apply inThere; apply_rules [h]; simp [h, renameComp]; rfl
+
+theorem wRenameSucc {Γ A} : Γ ∷ A ⊢ succ ∶ Γ := by
+  intro x B mem; constructor; assumption
+
+/-*------------------------------
+  Renaming and weakening lemmas
+------------------------------*-/
+
+theorem wtRename {ξ : ℕ → ℕ} {Γ Δ} {a A : Term}
+  (hξ : Δ ⊢ ξ ∶ Γ) (hΔ : ⊢ Δ) (h : Γ ⊢ a ∶ A) :
+  Δ ⊢ rename ξ a ∶ rename ξ A := by
+  generalize e : @Sigma.mk I idx I.wt ⟨Γ, a, A⟩ = t at h
+  induction h generalizing ξ Γ Δ a A
+  all_goals injection e with eI e; injection eI
+  all_goals injection e with eCtxt eTerm eType;
+            subst eCtxt; subst eTerm; subst eType
+  case var => constructor; assumption; apply_rules [hξ]
+  case 𝒰 ih => exact Wtf.𝒰 (ih hξ hΔ rfl)
+  case pi ihA ihB =>
+    let ihA' := ihA hξ hΔ rfl
+    refine Wtf.pi ihA' ?_
+    rw [renameLiftRename]
+    exact ihB (wRenameLift hξ) (Wtf.cons hΔ ihA') rfl
+  case abs ihPi ihb =>
+    let ihPi' := ihPi hξ hΔ rfl
+    refine Wtf.abs ihPi' ?_
+    let ⟨k, hA⟩ := wtfPiInvA ihPi'
+    exact ihb (wRenameLift hξ) (Wtf.cons hΔ hA) rfl
+  case app ihb iha => rw [← renameDist]; exact Wtf.app (ihb hξ hΔ rfl) (iha hξ hΔ rfl)
+  case mty ih => exact Wtf.mty (ih hξ hΔ rfl)
+  case exf ihA _ ihb => exact Wtf.exf (ihb hξ hΔ rfl) (ihA hξ hΔ rfl)
+  case lvl ih => exact Wtf.lvl (ih hξ hΔ rfl)
+  case lof => constructor <;> assumption
+  case trans ihi _ ihj => exact Wtf.trans (ihj hξ hΔ rfl) (ihi hξ hΔ rfl)
+  case conv B _ _ iha h _ ihA =>
+    exact Wtf.conv (convEqv (convRename ξ (eqvConv h))) (iha hξ hΔ rfl) (ihA hξ hΔ rfl)
+  case sub ihj _ ihA => exact Wtf.sub (ihj hξ hΔ rfl) (ihA hξ hΔ rfl)
+
+theorem wtWeaken {Γ k} {a A B : Term}
+  (hΓ : ⊢ Γ) (hB : Γ ⊢ B ∶ 𝒰 k) (h : Γ ⊢ a ∶ A) :
+  Γ ∷ B ⊢ rename succ a ∶ rename succ A := by
+  apply wtRename wRenameSucc (Wtf.cons hΓ hB) h
+
+/-*-------------------------
+  Well-typed substitutions
+-------------------------*-/
+
+def wSubst σ Γ Δ := ∀ x A, Γ ∋ x ∶ A → Δ ⊢ σ x ∶ subst σ A
+notation:40 Δ:41 "⊢" σ:41 "∶" Γ:41 => wSubst σ Γ Δ
+
+theorem wSubstUp {σ Δ Γ k A}
+  (hA : Δ ⊢ subst σ A ∶ 𝒰 k)
+  (h : Δ ⊢ σ ∶ Γ) :
+  Δ ∷ subst σ A ⊢ ⇑ σ ∶ Γ ∷ A := by
+  intro x B mem; cases mem
+  all_goals rw [← renameUpSubst]
+  . exact Wtf.var (Wtf.cons (wtWf hA) hA) In.here
+  . refine wtWeaken (wtWf hA) hA (h _ _ ?_); assumption
+
+theorem wSubstCons {Γ} {a A : Term}
+  (h : Γ ⊢ a ∶ A) :
+  Γ ⊢ a +: var ∶ Γ ∷ A := by
+  intro x B mem; cases mem
+  all_goals rw [← substDrop]
+  . exact h
+  . refine Wtf.var (wtWf h) ?_; assumption
+
+/-*---------------------------------
+  Morphing and substitution lemmas
+---------------------------------*-/
+
+theorem wtMorph {σ : ℕ → Term} {Γ Δ} {a A : Term}
+  (hσ : Δ ⊢ σ ∶ Γ) (hΔ : ⊢ Δ) (h : Γ ⊢ a ∶ A) :
+  Δ ⊢ subst σ a ∶ subst σ A := by
+  generalize e : @Sigma.mk I idx I.wt ⟨Γ, a, A⟩ = t at h
+  induction h generalizing σ Γ Δ a A
+  all_goals injection e with eI e; injection eI
+  all_goals injection e with eCtxt eTerm eType;
+            subst eCtxt; subst eTerm; subst eType
+  case var mem => exact hσ _ _ mem
+  case 𝒰 ih => exact Wtf.𝒰 (ih hσ hΔ rfl)
+  case pi ihA ihB =>
+    let ihA' := ihA hσ hΔ rfl
+    refine Wtf.pi ihA' ?_
+    rw [renameUpSubst]
+    exact ihB (wSubstUp ihA' hσ) (Wtf.cons hΔ ihA') rfl
+  case abs ihPi ihb =>
+    let ihPi' := ihPi hσ hΔ rfl
+    refine Wtf.abs ihPi' ?_
+    let ⟨k, hA⟩ := wtfPiInvA ihPi'
+    exact ihb (wSubstUp hA hσ) (Wtf.cons hΔ hA) rfl
+  case app ihb iha => rw [← substDist]; exact Wtf.app (ihb hσ hΔ rfl) (iha hσ hΔ rfl)
+  case mty ih => exact Wtf.mty (ih hσ hΔ rfl)
+  case exf ihA _ ihb => exact Wtf.exf (ihb hσ hΔ rfl) (ihA hσ hΔ rfl)
+  case lvl ih => exact Wtf.lvl (ih hσ hΔ rfl)
+  case lof => constructor <;> assumption
+  case trans ihi _ ihj => exact Wtf.trans (ihj hσ hΔ rfl) (ihi hσ hΔ rfl)
+  case conv B _ _ iha h _ ihA =>
+    refine Wtf.conv (convEqv (convSubst σ (eqvConv h))) (iha hσ hΔ rfl) (ihA hσ hΔ rfl)
+  case sub ihj _ ihA => exact Wtf.sub (ihj hσ hΔ rfl) (ihA hσ hΔ rfl)
+
+theorem wtSubst {Γ} {a A b B : Term}
+  (hb : Γ ⊢ b ∶ B) (h : Γ ∷ B ⊢ a ∶ A) :
+  Γ ⊢ subst (b +: var) a ∶ subst (b +: var) A := by
+  apply wtMorph (wSubstCons hb) (wtWf hb) h
+
+/-*-----------
+  Regularity
+-----------*-/
+
+theorem wtMem {Γ x A} (mem : Γ ∋ x ∶ A) (h : ⊢ Γ) : ∃ k, Γ ⊢ A ∶ 𝒰 k := by
+  induction mem
+  case here =>
+    cases h with
+    | cons hΓ hB =>
+      exact ⟨rename succ _, wtWeaken hΓ hB hB⟩
+  case there ih =>
+    cases h with
+    | cons hΓ hB =>
+      let ⟨k, hA⟩ := ih hΓ
+      exact ⟨rename succ k, wtWeaken hΓ hB hA⟩
+
+theorem wtRegularity {Γ} {a A : Term} (h : Γ ⊢ a ∶ A) : ∃ k, Γ ⊢ A ∶ 𝒰 k := by
+  generalize e : @Sigma.mk I idx I.wt ⟨Γ, a, A⟩ = t at h
+  induction h generalizing Γ a A
+  all_goals injection e with eI e; injection eI
+  all_goals injection e with eCtxt eTerm eType;
+            subst eCtxt; subst eTerm; subst eType
+  case var wf _ mem => exact wtMem mem wf
+  case 𝒰 j k _ ih =>
+    let ⟨_, ihk⟩ := ih rfl
+    let ⟨l, hk⟩ := wtfLvlInv ihk
+    exact ⟨l, Wtf.𝒰 hk⟩
+  case pi ihA _ => exact ihA rfl
+  case abs hPi _ _ _ => exact ⟨_, hPi⟩
+  case app ha ihb _ =>
+    let ⟨_, hPi⟩ := ihb rfl
+    let ⟨k, hB⟩ := wtfPiInvB hPi
+    exact ⟨subst _ k, wtSubst ha hB⟩
+  case mty hj _ => exact ⟨_, Wtf.𝒰 hj⟩
+  case exf hA _ => exact ⟨_, hA⟩
+  case lvl k ha _ =>
+    let ⟨l, klgt⟩ := exists_gt k
+    exact ⟨lof l, Wtf.𝒰 (Wtf.lof (wtWf ha) klgt)⟩
+  case lof k _ wf _ =>
+    let ⟨l, klgt⟩ := exists_gt k
+    exact ⟨lof l, Wtf.lvl (Wtf.lof wf klgt)⟩
+  case trans ih _ _ => exact ih rfl
+  case conv hA _ => exact ⟨_, hA⟩
+  case sub ih _ _ =>
+    let ⟨_, ihk⟩ := ih rfl
+    let ⟨l, hk⟩ := wtfLvlInv ihk
+    exact ⟨l, Wtf.𝒰 hk⟩
